theories/Bool/DecBool.v
@@ -10,7 +10,7 @@
 
 Set Implicit Arguments.
 
-Definition ifdec (A B:Prop) (C:Set) (H:{A} + {B}) (x y:C) : C :=
+Definition ifdec (A B:Prop) (C:Type) (H:{A} + {B}) (x y:C) : C :=
   if H then x else y.
 
 
