theories/Init/Notations.v
@@ -62,6 +62,9 @@ Reserved Notation "{ x }" (at level 0, x at level 99).
 
 (** Notations for sigma-types or subsets *)
 
+Reserved Notation "{ x  |  P }" (at level 0, x at level 99).
+Reserved Notation "{ x  |  P  &  Q }" (at level 0, x at level 99).
+
 Reserved Notation "{ x : A  |  P }" (at level 0, x at level 99).
 Reserved Notation "{ x : A  |  P  &  Q }" (at level 0, x at level 99).
 
